XmlOutput might now support reading one row variable

platform/XmlOutput.v
@@ -1,4 +1,5 @@
 Require Import AutoSep Wrap StringOps XmlLex SinglyLinkedList Malloc ArrayOps.
+Require Import RelDb RelDbSelect.
 
 Set Implicit Arguments.
 
@@ -8,7 +9,8 @@ Set Implicit Arguments.
 Inductive xml :=
 | Cdata (const : string)
 | Var (start len : string)
-| Tag (tag : string) (inner : list xml).
+| Tag (tag : string) (inner : list xml)
+| Column (data : string) (sch : schema) (col : string).
 
 Section ForallR.
   Variable A : Type.
@@ -48,6 +50,7 @@ Fixpoint wf (xm : xml) : Prop :=
     | Cdata const => goodSize (String.length const)
     | Var _ _ => True
     | Tag tag inner => goodSize (String.length tag + 3) /\ ForallR wf inner
+    | Column _ sch col => goodSize (length sch) /\ In col sch
   end.
 
 Fixpoint freeVar (xm : xml) (xs : string * string) : Prop :=
@@ -55,18 +58,16 @@ Fixpoint freeVar (xm : xml) (xs : string * string) : Prop :=
     | Cdata _ => False
     | Var start len => xs = (start, len)
     | Tag _ inner => ExistsR (fun xm' => freeVar xm' xs) inner
+    | Column _ _ _ => False
   end.
 
-Section mapConcat.
-  Variables A B : Type.
-  Variable f : A -> list B.
-
-  Fixpoint mapConcat (ls : list A) : list B :=
-    match ls with
-      | nil => nil
-      | x :: ls' => f x ++ mapConcat ls'
-    end.
-End mapConcat.
+Fixpoint freeRowVar (xm : xml) (xs : string * schema) : Prop :=
+  match xm with
+    | Cdata _ => False
+    | Var _ _ => False
+    | Tag _ inner => ExistsR (fun xm' => freeRowVar xm' xs) inner
+    | Column data sch _ => xs = (data, sch)
+  end.
 
 Section xml_ind'.
   Variable P : xml -> Prop.
@@ -77,6 +78,8 @@ Section xml_ind'.
 
   Hypothesis H_Tag : forall tag inner, List.Forall P inner -> P (Tag tag inner).
 
+  Hypothesis H_Column : forall data sch col, P (Column data sch col).
+
   Fixpoint xml_ind' (xm : xml) : P xm :=
     match xm with
       | Cdata const => H_Cdata const
@@ -86,6 +89,7 @@ Section xml_ind'.
           | nil => Forall_nil _
           | xm :: xms' => Forall_cons _ (xml_ind' xm) (xmls_ind xms')
         end) inner)
+      | Column data sch col => H_Column data sch col
     end.
 End xml_ind'.
 
@@ -95,6 +99,8 @@ Definition inBounds (cdatas : list (string * string)) (V : vals) :=
   List.Forall (fun p => wordToNat (V (fst p)) + wordToNat (V (snd p)) <= wordToNat (V "len"))%nat
   cdatas.
 
+Require Import Bags.
+
 
 (** * Compiling XML snippets into Bedrock chunks *)
 
@@ -103,17 +109,16 @@ Section Out.
   Variable invPre : A -> vals -> HProp.
   Variable invPost : A -> vals -> W -> HProp.
 
+  Variable data : string.
+  Variable sch : schema.
+
   (* Precondition and postcondition of generation *)
   Definition invar cdatas :=
     Al a : A, Al bsI, Al bsO,
-    PRE[V] array8 bsI (V "buf") * array8 bsO (V "obuf")
+    PRE[V] array8 bsI (V "buf") * array8 bsO (V "obuf") * row sch (V data)
       * [| length bsI = wordToNat (V "len") |] * [| length bsO = wordToNat (V "olen") |]
       * [| inBounds cdatas V |] * [| V "opos" <= V "olen" |] * invPre a V
     POST[R] Ex bsO', array8 bsI (V "buf") * array8 bsO' (V "obuf") * [| length bsO' = length bsO |] * invPost a V R.
-
-  (* Alternate sequencing operator, which generates twistier code but simpler postconditions and VCs *)
-  Definition SimpleSeq (ch1 ch2 : chunk) : chunk := fun ns res =>
-    Structured nil (fun im mn H => Seq_ H (toCmd ch1 mn H ns res) (toCmd ch2 mn H ns res)).
 
   Infix ";;" := SimpleSeq : SP_scope.
 
@@ -127,11 +132,20 @@ Section Out.
       end%SP.
   End OutList.
 
+  Fixpoint findCol (sch : schema) (s : string) : nat :=
+    match sch with
+      | nil => O
+      | s' :: sch' => if string_dec s s' then O else S (findCol sch' s)
+    end.
+
+  Inductive reveal_row : Prop := RevealRow.
+  Hint Constructors reveal_row.
+
   Fixpoint Out' (cdatas : list (string * string)) (xm : xml) : chunk :=
     match xm with
       | Cdata const => StringWrite "obuf" "olen" "opos" "overflowed" const
         (fun (p : list B * A) V => array8 (fst p) (V "buf") * [| length (fst p) = wordToNat (V "len") |]
-          * [| inBounds cdatas V |] * invPre (snd p) V)%Sep
+          * [| inBounds cdatas V |] * invPre (snd p) V * row sch (V data))%Sep
         (fun _ (p : list B * A) V R => Ex bs', array8 bs' (V "obuf") * [| length bs' = wordToNat (V "olen") |]
           * array8 (fst p) (V "buf") * invPost (snd p) V R)%Sep
       | Var start len =>
@@ -141,7 +155,7 @@ Section Out.
           [Al a : A, Al bsI, Al bsO,
             PRE[V] [| V len < V "olen" ^- V "opos" |]%word * array8 bsI (V "buf") * array8 bsO (V "obuf")
               * [| length bsI = wordToNat (V "len") |] * [| length bsO = wordToNat (V "olen") |]
-              * [| inBounds cdatas V |] * [| V "opos" <= V "olen" |]%word * invPre a V
+              * [| inBounds cdatas V |] * [| V "opos" <= V "olen" |]%word * invPre a V * row sch (V data)
             POST[R] Ex bsO', array8 bsI (V "buf") * array8 bsO' (V "obuf") * [| length bsO' = length bsO |]
               * invPost a V R];;
           "opos" <- "opos" + len
@@ -151,15 +165,89 @@ Section Out.
       | Tag tag inner =>
         StringWrite "obuf" "olen" "opos" "overflowed" ("<" ++ tag ++ ">")
         (fun (p : list B * A) V => array8 (fst p) (V "buf") * [| length (fst p) = wordToNat (V "len") |]
-          * invPre (snd p) V * [| inBounds cdatas V |])%Sep
+          * invPre (snd p) V * [| inBounds cdatas V |] * row sch (V data))%Sep
         (fun _ (p : list B * A) V R => Ex bs', array8 bs' (V "obuf") * [| length bs' = wordToNat (V "olen") |]
           * array8 (fst p) (V "buf") * invPost (snd p) V R)%Sep;;
         OutList (Out' cdatas) inner;;
         StringWrite "obuf" "olen" "opos" "overflowed" ("</" ++ tag ++ ">")
         (fun (p : list B * A) V => array8 (fst p) (V "buf") * [| length (fst p) = wordToNat (V "len") |]
-          * invPre (snd p) V * [| inBounds cdatas V |])%Sep
+          * invPre (snd p) V * [| inBounds cdatas V |] * row sch (V data))%Sep
         (fun _ (p : list B * A) V R => Ex bs', array8 bs' (V "obuf") * [| length bs' = wordToNat (V "olen") |]
           * array8 (fst p) (V "buf") * invPost (snd p) V R)%Sep
+      | Column data sch col =>
+        Note [reveal_row];;
+
+        Assert [Al a : A, Al bsI, Al bsO,
+          PRE[V] array8 bsI (V "buf") * array8 bsO (V "obuf")
+            * [| length bsI = wordToNat (V "len") |] * [| length bsO = wordToNat (V "olen") |]
+            * [| inBounds cdatas V |] * [| V "opos" <= V "olen" |]%word * invPre a V
+            * Ex buf, Ex len, Ex cols, Ex bs,
+              (V data ==*> buf, len) * array (posl cols) (V data ^+ $8)
+              * array (lenl cols) (V data ^+ $8 ^+ $(length sch * 4)) * array8 bs buf
+              * [| length bs = wordToNat len |] * [| length cols = length sch |] * [| RelDb.inBounds len cols |]
+              * [| V data <> 0 |] * [| freeable (V data) (2 + length sch + length sch) |]
+              * [| buf <> 0 |] * [| freeable8 buf (length bs) |]
+              * [| natToW (findCol sch col) < natToW (length (lenl cols)) |]%word
+          POST[R] Ex bsO', array8 bsI (V "buf") * array8 bsO' (V "obuf")
+            * [| length bsO' = length bsO |] * invPost a V R];;
+
+        "matched" <- data + 8;;
+        "matched" <- "matched" + (length sch * 4)%nat;;
+        "matched" <-* "matched" + (4 * findCol sch col)%nat;;
+
+        "tmp" <- "olen" - "opos";;
+        If ("matched" < "tmp") {
+          Assert [Al a : A, Al bsI, Al bsO,
+            PRE[V] array8 bsI (V "buf") * array8 bsO (V "obuf")
+              * [| length bsI = wordToNat (V "len") |] * [| length bsO = wordToNat (V "olen") |]
+              * [| inBounds cdatas V |] * [| V "opos" <= V "olen" |]%word * invPre a V
+              * Ex buf, Ex len, Ex cols, Ex bs,
+                (V data ==*> buf, len) * array (posl cols) (V data ^+ $8)
+                * array (lenl cols) (V data ^+ $8 ^+ $(length sch * 4)) * array8 bs buf
+                * [| length bs = wordToNat len |] * [| length cols = length sch |] * [| RelDb.inBounds len cols |]
+                * [| V data <> 0 |] * [| freeable (V data) (2 + length sch + length sch) |]
+                * [| buf <> 0 |] * [| freeable8 buf (length bs) |]
+                * [| V "matched" = Array.selN (lenl cols) (findCol sch col) |]
+                * [| natToW (findCol sch col) < natToW (length (posl cols)) |]%word
+                * [| V "matched" < V "olen" ^- V "opos" |]%word
+            POST[R] Ex bsO', array8 bsI (V "buf") * array8 bsO' (V "obuf")
+              * [| length bsO' = length bsO |] * invPost a V R];;
+
+          "tmp" <- data + 8;;
+          "tmp" <-* "tmp" + (4 * findCol sch col)%nat;;
+
+          Assert [Al a : A, Al bsI, Al bsO,
+            PRE[V] array8 bsI (V "buf") * array8 bsO (V "obuf")
+              * [| length bsI = wordToNat (V "len") |] * [| length bsO = wordToNat (V "olen") |]
+              * [| inBounds cdatas V |] * [| V "opos" <= V "olen" |]%word * invPre a V
+              * Ex buf, Ex len, Ex cols, Ex bs,
+                (V data ==*> buf, len) * array (posl cols) (V data ^+ $8)
+                * array (lenl cols) (V data ^+ $8 ^+ $(length sch * 4)) * array8 bs buf
+                * [| length bs = wordToNat len |] * [| length cols = length sch |] * [| RelDb.inBounds len cols |]
+                * [| V data <> 0 |] * [| freeable (V data) (2 + length sch + length sch) |]
+                * [| buf <> 0 |] * [| freeable8 buf (length bs) |]
+                * [| V "matched" = Array.selN (lenl cols) (findCol sch col) |]
+                * [| V "tmp" = Array.selN (posl cols) (findCol sch col) |]
+                * [| V "matched" < V "olen" ^- V "opos" |]%word
+            POST[R] Ex bsO', array8 bsI (V "buf") * array8 bsO' (V "obuf")
+              * [| length bsO' = length bsO |] * invPost a V R];;
+
+          Note [reveal_row];;
+          "res" <-* data;;
+
+          Call "array8"!"copy"("obuf", "opos", "res", "tmp", "matched")
+          [Al a : A, Al bsI, Al bsO,
+            PRE[V] [| V "matched" < V "olen" ^- V "opos" |]%word * array8 bsI (V "buf") * array8 bsO (V "obuf")
+              * [| length bsI = wordToNat (V "len") |] * [| length bsO = wordToNat (V "olen") |]
+              * [| inBounds cdatas V |] * [| V "opos" <= V "olen" |]%word * invPre a V * row sch (V data)
+            POST[R] Ex bsO', array8 bsI (V "buf") * array8 bsO' (V "obuf") * [| length bsO' = length bsO |]
+              * invPost a V R];;
+          "opos" <- "opos" + "matched"
+        } else {
+          Note [reveal_row];;
+
+          "overflowed" <- 1
+        }
     end%SP.
 
   Opaque mult.
@@ -201,8 +289,10 @@ Section Out.
   Qed.
 
   Definition cdatasGood (cdatas : list (string * string)) :=
-    List.Forall (fun p => fst p <> "opos" /\ fst p <> "overflowed" /\ fst p <> "tmp"
-      /\ snd p <> "opos" /\ snd p <> "overflowed" /\ snd p <> "tmp") cdatas.
+    List.Forall (fun p => fst p <> "opos" /\ fst p <> "overflowed" /\ fst p <> "tmp" /\ fst p <> "matched"
+      /\ fst p <> "res"
+      /\ snd p <> "opos" /\ snd p <> "overflowed" /\ snd p <> "tmp" /\ snd p <> "matched"
+      /\ snd p <> "res") cdatas.
 
   Ltac prepl := post; unfold lvalIn, regInL, immInR in *;
     repeat match goal with
@@ -216,7 +306,8 @@ Section Out.
     try match goal with
           | [ H : cdatasGood _, H' : In _ _ |- _ ] =>
             specialize (proj1 (Forall_forall _ _) H _ H'); simpl; intuition idtac
-        end.
+        end;
+    try rewrite natToW_4times in *.
 
   Ltac my_descend :=
     try match goal with
@@ -228,7 +319,11 @@ Section Out.
     repeat match goal with
              | [ H : evalInstrs _ _ _ = _ |- _ ] => clear H
              | [ H : evalCond _ _ _ _ _ = _ |- _ ] => clear H
-             | [ H : In _ _ |- _ ] => clear H
+             | [ H : In _ ?ls |- _ ] =>
+               match ls with
+                 | sch => fail 1
+                 | _ => clear H
+               end
              | [ x : (_ * _)%type |- _ ] => destruct x; simpl in *
            end;
     unfold invar, localsInvariant; descend;
@@ -294,11 +389,18 @@ Section Out.
             end
         end;
 
-    step auto_ext.
+    match goal with
+      | _ => weaken_invPre
+      | [ _ : context[reveal_row] |- _ ] => try match_locals; step RelDb.hints
+      | _ => try match_locals; step auto_ext
+    end.
 
   Ltac t := post; repeat invoke1; prep; propxFo;
     repeat invoke1; prepl;
-      evaluate auto_ext; my_descend; (repeat (bash; my_descend); eauto).
+      match goal with
+        | [ _ : context[reveal_row] |- _ ] => evaluate RelDb.hints
+        | _ => evaluate auto_ext
+      end; my_descend; (repeat (bash; my_descend); eauto).
 
   Notation "l ~~ im ~~> s" := (LabelMap.find l%SP im = Some (Precondition s None)) (at level 0).
 
@@ -312,11 +414,24 @@ Section Out.
     Hypothesis Hoverflowed : In "overflowed" ns.
     Hypothesis Htmp : In "tmp" ns.
     Hypothesis Hbuf : In "buf" ns.
+    Hypothesis Hmatched : In "matched" ns.
+    Hypothesis HresV : In "res" ns.
+    Hypothesis Hdata : In data ns.
+
+    Hypothesis Hnot_rp : data <> "rp".
+    Hypothesis Hnot_obuf : data <> "obuf".
+    Hypothesis Hnot_opos : data <> "opos".
+    Hypothesis Hnot_overflowed : data <> "overflowed".
+    Hypothesis Hnot_tmp : data <> "tmp".
+    Hypothesis Hnot_buf : data <> "buf".
+    Hypothesis Hnot_matched : data <> "matched".
+    Hypothesis Hnot_res : data <> "res".
+
     Hypothesis HinvPre : forall a V V', (forall x, x <> "overflowed" -> x <> "opos" -> x <> "tmp"
-      -> sel V x = sel V' x)
+      -> x <> "matched" -> x <> "res" -> sel V x = sel V' x)
     -> invPre a V ===> invPre a V'.
     Hypothesis HinvPost : forall a V V' R, (forall x, x <> "overflowed" -> x <> "opos" -> x <> "tmp"
-      -> sel V x = sel V' x)
+      -> x <> "matched" -> x <> "res" -> sel V x = sel V' x)
     -> invPost a V R = invPost a V' R.
     Hypothesis Hres : (res >= 7)%nat.
 
@@ -330,6 +445,9 @@ Section Out.
         | [ H : forall start len : string, _ |- _ ] =>
           generalize (fun start len H' => H start len (or_introl _ H'));
             specialize (fun start len H' => H start len (or_intror _ H')); intro
+        | [ H : forall (data : string) (sch : schema), _ |- _ ] =>
+          generalize (fun start len H' => H start len (or_introl _ H'));
+            specialize (fun start len H' => H start len (or_intror _ H')); intro
       end.
 
     Lemma OutList_correct : forall cdatas, cdatasGood cdatas
@@ -340,6 +458,7 @@ Section Out.
           -> (forall start len, freeVar xm (start, len) -> In start ns /\ In len ns)
           -> (forall specs st, interp specs (pre st)
             -> interp specs (invar cdatas true (fun x => x) ns res st))
+          -> (forall data' sch', freeRowVar xm (data', sch') -> data' = data /\ sch' = sch)
           -> (forall specs st,
             interp specs (Postcondition (toCmd (Out' cdatas xm) mn H ns res pre) st)
             -> interp specs (invar cdatas true (fun x => x) ns res st))
@@ -350,6 +469,7 @@ Section Out.
           -> (forall start len, ExistsR (fun xm => freeVar xm (start, len)) xms -> In start ns /\ In len ns)
           -> (forall specs st, interp specs (pre st)
             -> interp specs (invar cdatas true (fun x => x) ns res st))
+          -> (forall data' sch', ExistsR (fun xm => freeRowVar xm (data', sch')) xms -> data' = data /\ sch' = sch)
           -> (forall specs st, interp specs (Postcondition (toCmd (OutList (Out' cdatas) xms) mn H ns res pre) st)
             -> interp specs (invar cdatas true (fun x => x) ns res st))
           /\ vcs (VerifCond (toCmd (OutList (Out' cdatas) xms) mn H ns res pre)).
@@ -377,7 +497,8 @@ Section Out.
     Lemma inBounds_weaken : forall cdatas V V',
       cdatasGood cdatas
       -> inBounds cdatas V
-      -> (forall x, x <> "overflowed" -> x <> "opos" -> x <> "tmp" -> sel V x = sel V' x)
+      -> (forall x, x <> "overflowed" -> x <> "opos" -> x <> "tmp" -> x <> "matched"
+        -> x <> "res" -> sel V x = sel V' x)
       -> inBounds cdatas V'.
       intros; rewrite <- inBounds_sel in *;
         eapply Forall_impl2; [ match goal with
@@ -398,6 +519,8 @@ Section Out.
     Ltac deDouble :=
       repeat match goal with
                | [ H : forall start len : string, _ |- _ ] =>
+                   specialize (H _ _ eq_refl)
+               | [ H : forall (data' : string) (sch' : schema), _ |- _ ] =>
                    specialize (H _ _ eq_refl)
              end.
 
@@ -434,7 +557,6 @@ Section Out.
       -> c ^+ a <= b.
       clear; intros.
       pre_nomega.
-      rewrite wordToNat_wminus in * by nomega.
       rewrite wordToNat_wplus in *.
       omega.
       apply goodSize_weaken with (wordToNat b); eauto.
@@ -460,7 +582,6 @@ Section Out.
       -> (wordToNat c + wordToNat a <= n)%nat.
       clear; intros; subst.
       pre_nomega.
-      rewrite wordToNat_wminus in * by nomega.
       omega.
     Qed.
 
@@ -472,6 +593,93 @@ Section Out.
 
     Hint Rewrite wplus_wminus mult4_S : sepFormula.
 
+    Lemma findCol_bound : forall s col,
+      In col s
+      -> (findCol s col < length s)%nat.
+      clear; induction s; simpl; intuition subst;
+        match goal with
+          | [ |- context[if ?E then _ else _] ] => destruct E
+        end; intuition.
+    Qed.
+
+    Lemma findCol_bound_natToW : forall col n,
+      In col sch
+      -> goodSize (Datatypes.length sch)
+      -> n = length sch
+      -> natToW (findCol sch col) < natToW n.
+      clear; intros; subst.
+      pre_nomega.
+      rewrite wordToNat_natToWord_idempotent.
+      rewrite wordToNat_natToWord_idempotent.
+      eauto using findCol_bound.
+      apply findCol_bound in H; congruence.
+      change (goodSize (findCol sch col)); eapply goodSize_weaken; eauto.
+      apply findCol_bound in H; auto.
+    Qed.
+
+    Lemma findCol_posl : forall col cols,
+      In col sch
+      -> goodSize (Datatypes.length sch)
+      -> length cols = length sch
+      -> natToW (findCol sch col) < natToW (length (posl cols)).
+      intros; rewrite length_posl; eauto using findCol_bound_natToW.
+    Qed.
+
+    Lemma findCol_lenl : forall col cols,
+      In col sch
+      -> goodSize (Datatypes.length sch)
+      -> length cols = length sch
+      -> natToW (findCol sch col) < natToW (length (lenl cols)).
+      intros; rewrite length_lenl; eauto using findCol_bound_natToW.
+    Qed.
+
+    Hint Immediate findCol_posl findCol_lenl.
+
+    Lemma selN_col : forall col cols,
+      In col sch
+      -> goodSize (length sch)
+      -> length cols = length sch
+      -> Array.sel cols (natToW (findCol sch col)) = selN cols (findCol sch col).
+      clear; unfold Array.sel; intros; f_equal.
+      apply wordToNat_natToWord_idempotent.
+      change (goodSize (findCol sch col)).
+      eapply goodSize_weaken; eauto.
+      apply findCol_bound in H; auto.
+    Qed.
+
+    Lemma selN_posl : forall col cols,
+      In col sch
+      -> goodSize (length sch)
+      -> length cols = length sch
+      -> Array.sel (posl cols) (natToW (findCol sch col)) = selN (posl cols) (findCol sch col).
+      intros; apply selN_col; auto; rewrite length_posl; auto.
+    Qed.
+
+    Lemma selN_lenl : forall col cols,
+      In col sch
+      -> goodSize (length sch)
+      -> length cols = length sch
+      -> Array.sel (lenl cols) (natToW (findCol sch col)) = selN (lenl cols) (findCol sch col).
+      intros; apply selN_col; auto; rewrite length_lenl; auto.
+    Qed.
+
+    Hint Immediate selN_posl selN_lenl.
+
+    Lemma inBounds_selN : forall len cols,
+      RelDb.inBounds len cols
+      -> forall col a b c, a = selN (posl cols) (findCol sch col)
+        -> b = selN (lenl cols) (findCol sch col)
+        -> c = wordToNat len
+        -> In col sch
+        -> length cols = length sch
+        -> (wordToNat a + wordToNat b <= c)%nat.
+      intros; eapply inBounds_selN; try eassumption.
+      rewrite H5; eapply findCol_bound; auto.
+    Qed.
+
+    Hint Extern 1 (_ + _ <= _)%nat =>
+      eapply inBounds_selN; try eassumption; (cbv beta; congruence).
+
     Lemma Out_correct : forall cdatas, cdatasGood cdatas
       -> "array8"!"copy" ~~ im ~~> copyS
       -> forall xm pre,
@@ -480,31 +688,42 @@ Section Out.
         -> (forall start len, freeVar xm (start, len) -> In start ns /\ In len ns)
         -> (forall specs st, interp specs (pre st)
           -> interp specs (invar cdatas true (fun x => x) ns res st))
+        -> (forall data' sch', freeRowVar xm (data', sch') -> data' = data /\ sch' = sch)
         -> (forall specs st, interp specs (Postcondition (toCmd (Out' cdatas xm) mn H ns res pre) st)
           -> interp specs (invar cdatas true (fun x => x) ns res st))
         /\ vcs (VerifCond (toCmd (Out' cdatas xm) mn H ns res pre)).
       induction xm using xml_ind'; (post; try match goal with
                                                 | [ |- vcs (_ :: _) ] => wrap0; try discriminate
-                                              end; deDouble; deSpec);
+                                              end; deDouble; deSpec; intuition subst);
       abstract solve [ t | proveHimp |
         match goal with
           | [ H : List.Forall _ _ |- _ ] =>
-            eapply OutList_correct in H; [ destruct H; eauto | auto | auto | auto | auto | ]
+            eapply OutList_correct in H; [ destruct H; eauto | auto | auto | auto | auto | auto | | auto ]
         end; t ].
     Qed.
   End Out_correct.
 
   Notation OutVcs cdatas xm := (fun im ns res =>
     (~In "rp" ns) :: In "obuf" ns :: In "olen" ns :: In "opos" ns :: In "overflowed" ns
-    :: In "tmp" ns :: In "buf" ns
-    :: (forall a V V', (forall x, x <> "overflowed" -> x <> "opos" -> x <> "tmp" -> sel V x = sel V' x)
+    :: In "tmp" ns :: In "buf" ns :: In "matched" ns :: In "res" ns :: In data ns
+    :: (data <> "rp")%type
+    :: (data <> "obuf")%type
+    :: (data <> "opos")%type
+    :: (data <> "overflowed")%type
+    :: (data <> "tmp")%type
+    :: (data <> "buf")%type
+    :: (data <> "matched")%type
+    :: (data <> "res")%type
+    :: (forall a V V', (forall x, x <> "overflowed" -> x <> "opos" -> x <> "tmp"
+      -> x <> "matched" -> x <> "res" -> sel V x = sel V' x)
       -> invPre a V ===> invPre a V')
     :: (forall a V V' R, (forall x, x <> "overflowed" -> x <> "opos" -> x <> "tmp" -> sel V x = sel V' x)
-      -> invPost a V R = invPost a V' R)
+      -> x <> "matched" -> x <> "res" -> invPost a V R = invPost a V' R)
     :: (res >= 7)%nat
     :: wf xm
     :: (forall start len, freeVar xm (start, len) -> In (start, len) cdatas)
     :: (forall start len, freeVar xm (start, len) -> In start ns /\ In len ns)
+    :: (forall data' sch', freeRowVar xm (data', sch') -> data' = data /\ sch' = sch)
     :: cdatasGood cdatas
     :: "array8"!"copy" ~~ im ~~> copyS
     :: nil).
